theories/Parallel/Contract.v
@@ -1,0 +1,544 @@
+Require Import Lists.List.
+Require Import FunInd.
+Require Import Bool.Bool.
+Require Import Bool.Sumbool.
+Require Import Structures.GenericMinMax.
+From Equations Require Import Equations.
+Import ListNotations.
+Require Import micromega.Lia.
+Require Import Setoid.
+Require Import Init.Tauto btauto.Btauto.
+Require Import Logic.ClassicalFacts.
+
+(** printing =~ %$=\sim$% *)
+
+Set Implicit Arguments.
+
+
+
+
+Inductive EventType : Type :=
+| Transfer : EventType
+| Notify : EventType.
+
+Scheme Equality for EventType.
+
+
+Definition Trace := List.list EventType % type.
+
+Inductive Contract : Set :=
+| Success : Contract
+| Failure : Contract
+| Event : EventType -> Contract
+| CPlus : Contract -> Contract -> Contract
+| CSeq : Contract -> Contract -> Contract
+| Par : Contract -> Contract -> Contract.
+
+
+
+Notation "c0 _;_ c1"  := (CSeq c0 c1)
+                         (at level 50, left associativity).
+
+Notation "c0 _*_ c1"  := (Par c0 c1)
+                         (at level 52, left associativity).
+
+Notation "c0 _+_ c1"  := (CPlus c0 c1)
+                         (at level 53, left associativity).
+
+Scheme Equality for Contract.
+
+
+Fixpoint nu(c:Contract):bool :=
+match c with
+| Success => true
+| Failure => false
+| Event e => false
+| c0 _;_ c1 => nu c0 && nu c1
+| c0 _+_ c1 => nu c0 || nu c1
+| c0 _*_ c1 => nu c0 && nu c1
+end.
+
+Definition o (c : Contract) := if nu c then Success else Failure.
+Hint Unfold o : core.
+
+Lemma o_Failure : o Failure = Failure.
+Proof. reflexivity.
+Qed.
+
+Lemma o_Success : o Success = Success.
+Proof. reflexivity.
+Qed.
+
+
+Lemma o_or : forall (c : Contract), o c = Success /\ nu c = true \/ o c = Failure /\ nu c = false.
+Proof.
+intros. unfold o. destruct (nu c) eqn:Heqn; intuition.
+Qed.
+
+Lemma o_idempotent : forall (c : Contract), o (o c) = o c.
+Proof.
+intros. destruct (o_or c). destruct H. rewrite H;auto. destruct H. now rewrite H. 
+Qed.
+
+Hint Rewrite o_Failure o_Success o_idempotent : cDB.
+
+Reserved Notation "e \ c" (at level 40, left associativity).
+Fixpoint derive (e:EventType) (c:Contract) :Contract :=
+match c with
+| Success => Failure
+| Failure => Failure
+| Event e' => if (EventType_eq_dec e' e) then Success else Failure
+| c0 _;_ c1 => o c0 _;_ e \ c1 _+_ e \ c0 _;_ c1
+| c0 _+_ c1 => e \ c0 _+_ e \ c1
+| c0 _*_ c1 => (derive e c0) _*_ c1 _+_ c0 _*_ (derive e c1)
+end
+where "e \ c" := (derive e c).
+
+Ltac destruct_ctx :=
+  repeat match goal with
+         | [ H: ?H0 /\ ?H1 |- _ ] => destruct H
+         | [ H: exists _, _  |- _ ] => destruct H
+         end.
+
+Ltac o_destruct :=
+  match goal with
+         | [ |- context[(o ?c)] ] => destruct (o_or c);destruct_ctx
+         | [ _ : context[ (o ?c)] |- _ ] => let H := fresh "H" in 
+                                            let H1 := fresh "H1" in 
+                                            destruct (o_or c) as [[H H1] | [H H1]];
+                                            rewrite H in*;clear H
+         end.
+
+Lemma o_derive : forall c e, e \ (o c) = Failure.
+Proof.
+intros. o_destruct. unfold o. rewrite H0. now simpl. unfold o. rewrite H0. now simpl.
+Qed.
+
+Hint Rewrite o_idempotent o_derive : cDB.
+Ltac autoIC := auto with cDB.
+
+
+(*Removed because it is not needed in this file*)
+(*
+Inductive Trace_Derive : Contract -> Trace -> Contract -> Prop :=
+| Trace_Derive_Nil c : Trace_Derive c [] c
+| Trace_Derive_Cons c s c' e (H: Trace_Derive (c/e) s c') : Trace_Derive c (e::s) c'. (*rule motivated by constructor being analgous to cons on lists*)
+Hint Constructors Trace_Derive : cDB.
+
+
+Lemma Trace_Derive_trans : forall s s' c0 c1 c2 , Trace_Derive c0 s c1 -> Trace_Derive c1 s' c2 -> Trace_Derive c0 (s++s') c2.
+Proof.
+intros. induction H;simpl;autoIC.
+Qed.*)
+
+
+Reserved Notation "s \\ c" (at level 42, no associativity).
+Fixpoint trace_derive (s : Trace) (c : Contract)  : Contract :=
+match s with
+| [] => c
+| e::s' => s' \\ (e \ c)
+end
+where "s \\ c" := (trace_derive s c).
+
+
+Inductive interleave (A : Set) : list A -> list A -> list A -> Prop :=
+| IntLeftNil t : interleave nil t t
+| IntRightNil t : interleave t nil t
+| IntLeftCons t1 t2 t3 e (H: interleave t1 t2 t3) : interleave (e :: t1) t2 (e :: t3)
+| IntRightCons t1 t2 t3 e (H: interleave t1 t2 t3) : interleave t1 (e :: t2) (e :: t3).
+Hint Constructors interleave : cDB.
+
+
+
+
+
+Fixpoint interleave_fun (A : Set) (l0 l1 l2 : list A ) : Prop :=
+match l2 with
+| [] => l0 = [] /\ l1 = []
+| a2::l2' => match l0 with
+            | [] => l1 = l2
+            | a0::l0' => a2=a0 /\ interleave_fun l0' l1 l2' \/ match l1 with
+                                                           | [] => l0 = l2
+                                                           | a1::l1' => a2=a1 /\ interleave_fun l0 l1' l2'
+                                                           end
+            end
+end.
+
+Lemma interl_fun_nil : forall (A:Set), @interleave_fun A [] [] [].
+Proof. intros. unfold interleave_fun. split;auto. Qed.
+
+Hint Resolve interl_fun_nil : cDB.
+
+Lemma interl_fun_l : forall (A:Set) (l : list A), interleave_fun l [] l.
+Proof.
+induction l;intros; auto with cDB. simpl. now right.
+Qed.
+
+Lemma interl_fun_r : forall (A:Set) (l : list A), interleave_fun [] l  l.
+Proof.
+induction l;intros; auto with cDB. now simpl. 
+Qed.
+
+Hint Resolve interl_fun_l interl_fun_r : cDB.
+
+
+
+Lemma interl_eq_l : forall (A: Set) (l0 l1 : list A), interleave [] l0 l1 -> l0 = l1.
+Proof.
+induction l0;intros;simpl.
+- inversion H;auto.
+- inversion H; subst; auto. f_equal. auto. 
+Qed.
+
+Lemma interl_comm : forall (A: Set) (l0 l1 l2 : list A), interleave l0 l1 l2 -> interleave l1 l0 l2.
+Proof.
+intros. induction H;auto with cDB.
+Qed.
+
+Lemma interl_eq_r : forall (A: Set) (l0 l1 : list A), interleave  l0 [] l1 -> l0 = l1.
+Proof. auto using interl_eq_l,interl_comm.
+Qed.
+
+Lemma interl_nil : forall (A: Set) (l0 l1 : list A), interleave  l0 l1 [] -> l0 = [] /\ l1 = [].
+Proof.
+intros. inversion H;subst; split;auto.
+Qed.
+
+Lemma interl_or : forall (A:Set)(l2 l0 l1 :list A)(a0 a1 a2:A), interleave (a0::l0) (a1::l1) (a2 :: l2) -> a0 = a2 \/ a1 = a2.
+Proof.
+intros. inversion H;subst; auto||auto.
+Qed.
+
+Lemma interl_i_fun : forall (A:Set)(l0 l1 l2 : list A), interleave l0 l1 l2 -> interleave_fun l0 l1 l2.
+Proof.
+intros. induction H;auto with cDB.
+- simpl. left. split;auto.
+- simpl. destruct t1. apply interl_eq_l in H. now subst. right. split;auto.
+Qed.
+
+Lemma fun_i_interl : forall (A:Set)(l2 l0 l1 : list A), interleave_fun l0 l1 l2 -> interleave l0 l1 l2.
+Proof.
+induction l2;intros.
+- simpl in*. destruct H. subst. constructor.
+- simpl in H. destruct l0. subst. auto with cDB.
+  destruct H.
+  * destruct H. subst. auto with cDB.
+  * destruct l1.
+    ** inversion H. auto with cDB.
+    ** destruct H. subst. auto with cDB.
+Qed.
+
+Theorem interl_iff_fun : forall (A:Set)(l2 l0 l1 : list A), interleave l0 l1 l2 <-> interleave_fun l0 l1 l2.
+Proof. split;auto using interl_i_fun,fun_i_interl.
+Qed.
+
+Lemma interl_eq_r_fun : forall (A: Set) (l0 l1 : list A), interleave_fun  l0 [] l1 -> l0 = l1.
+Proof. intros. rewrite <- interl_iff_fun in H. auto using interl_eq_r.
+Qed.
+
+Lemma interl_eq_l_fun : forall (A: Set) (l0 l1 : list A), interleave_fun  [] l0 l1 -> l0 = l1.
+Proof. intros. rewrite <- interl_iff_fun in H. auto using interl_eq_l.
+Qed.
+
+Lemma interl_fun_cons_l : forall (A: Set) (a:A) (l0 l1 l2 : list A), interleave_fun l0 l1 l2 ->
+interleave_fun (a::l0) l1 (a::l2).
+Proof. intros. rewrite <- interl_iff_fun in *. auto with cDB. 
+Qed.
+
+Lemma interl_fun_cons_r : forall (A: Set) (a:A) (l0 l1 l2 : list A), interleave_fun l0 l1 l2 ->
+interleave_fun l0 (a::l1) (a::l2).
+Proof. intros. rewrite <- interl_iff_fun in *. auto with cDB. 
+Qed.
+
+Hint Rewrite interl_eq_r interl_eq_l interl_eq_r_fun interl_eq_l_fun : cDB.
+
+Hint Resolve interl_fun_cons_l interl_fun_cons_r : cDB.
+
+Ltac interl_tac := 
+        (repeat match goal with
+         | [ H: _::_ = [] |- _ ] => discriminate
+         | [ H: _ /\ _ |- _ ] => destruct H
+         | [ H: _ \/ _ |- _ ] => destruct H
+         | [ H: interleave_fun _ _ [] |- _ ] => simpl in H
+         | [ H: interleave_fun _ _ (?e::?s) |- _ ] => simpl in H
+         | [ H: interleave_fun _ _ ?s |- _ ] => destruct s;simpl in H
+         | [ H: interleave _ _ _ |- _ ] => rewrite interl_iff_fun in H
+         end);subst.
+
+Lemma interl_fun_app : forall (l l0 l1 l_interl l2  : Trace),
+interleave_fun l0 l1 l_interl -> interleave_fun l_interl l2 l -> 
+exists l_interl', interleave_fun l1 l2 l_interl' /\ interleave_fun l0 l_interl' l.
+Proof.
+induction l;intros.
+- simpl in H0. destruct H0. subst. simpl in H. destruct H.
+  subst.  exists []. split;auto with cDB.
+- simpl in H0. destruct l_interl. simpl in H. destruct H. subst.
+  exists (a::l). split;auto with cDB.
+  destruct H0.
+  * destruct H0. subst. simpl in H. destruct l0.
+    ** subst. exists (e::l). split;auto with cDB.
+    ** destruct H. destruct H. subst.
+      *** eapply IHl in H1;eauto. destruct_ctx.
+          exists x. split;auto with cDB.
+      *** destruct l1.
+        **** inversion H. subst. exists l2.
+             split;auto with cDB.
+        **** destruct H. subst. eapply IHl in H1;eauto. destruct_ctx.
+             exists (e1::x). split;auto with cDB;
+             apply interl_iff_fun; constructor;
+         now rewrite interl_iff_fun.
+  * destruct l2.
+    ** inversion H0. subst. exists l1. split; auto with cDB.
+    ** destruct H0. subst. eapply IHl in H1;eauto. destruct H1.
+       exists (e0::x). split; apply interl_iff_fun; constructor;
+       destruct H0; now rewrite interl_iff_fun.
+Qed.
+
+Lemma interl_app : forall (l l0 l1 l_interl l2  : Trace),
+interleave l0 l1 l_interl -> interleave l_interl l2 l -> 
+exists l_interl', interleave l1 l2 l_interl' /\ interleave l0 l_interl' l.
+Proof.
+intros. rewrite interl_iff_fun in *.
+eapply interl_fun_app in H0;eauto. destruct_ctx. exists x.
+repeat rewrite interl_iff_fun. split;auto.
+Qed.
+
+
+
+Lemma event_interl : forall s (e0 e1 : EventType), interleave_fun [e0] [e1] s -> s = [e0]++[e1] \/ s = [e1]++[e0].
+Proof.
+induction s;intros. simpl in H. destruct H. discriminate.
+simpl in H. destruct H.
+- destruct H. subst. apply interl_eq_l_fun in H0. subst.
+  now left.
+- destruct H. subst. apply interl_eq_r_fun in H0. subst.
+  now right.
+Qed.
+
+Lemma interleave_app : forall (A:Set) (s0 s1: list A), interleave s0 s1 (s0++s1).
+Proof.
+induction s0;intros;simpl;auto with cDB.
+Qed.
+
+Hint Resolve interleave_app : cDB.
+
+Lemma interleave_app2 : forall (A:Set) (s1 s0: list A), interleave s0 s1 (s1++s0).
+Proof.
+induction s1;intros;simpl;auto with cDB.
+Qed.
+
+Hint Resolve interleave_app interleave_app2 : cDB.
+
+Lemma interl_extend_r : forall (l0 l1 l2 l3 : Trace),
+interleave l0 l1 l2 -> interleave l0 (l1++l3) (l2++l3). 
+Proof.
+intros. generalize dependent l3. induction H;intros;simpl;auto with cDB.
+Qed.
+
+Lemma interl_extend_l : forall (l0 l1 l2 l3 : Trace),
+interleave l0 l1 l2 -> interleave (l0++l3) l1 (l2++l3). 
+Proof.
+intros. generalize dependent l3. induction H;intros;simpl;auto with cDB.
+Qed.
+
+
+Reserved Notation "s =~ re" (at level 63).
+Inductive Matches_Comp : Trace -> Contract -> Prop :=
+  | MSuccess : [] =~ Success
+  | MEvent x : [x] =~ (Event x)
+  | MSeq s1 c1 s2 c2
+             (H1 : s1 =~ c1)
+             (H2 : s2 =~ c2)
+           : (s1 ++ s2) =~ (c1 _;_ c2)
+  | MPlusL s1 c1 c2
+                (H1 : s1 =~ c1)
+              : s1 =~ (c1 _+_ c2)
+  | MPlusR c1 s2 c2
+                (H2 : s2 =~ c2)
+              : s2 =~ (c1 _+_ c2)
+  | MPar s1 c1 s2 c2 s
+             (H1 : s1 =~ c1)
+             (H2 : s2 =~ c2)
+             (H3 : interleave s1 s2 s)
+           : s =~ (c1 _*_ c2)
+  where "s =~ c" := (Matches_Comp s c).
+
+(*Derive Signature for Matches_Comp.*)
+
+Hint Constructors Matches_Comp : cDB.
+
+Ltac eq_event_destruct :=
+  repeat match goal with
+         | [ |- context[EventType_eq_dec ?e ?e0] ] => destruct (EventType_eq_dec e e0);try contradiction
+         | [ _ : context[EventType_eq_dec ?e ?e0]  |- _ ] => destruct (EventType_eq_dec e e0);try contradiction
+         end.
+
+Lemma seq_Success : forall c s, s =~ Success _;_ c <-> s =~ c.
+Proof.
+split;intros. inversion H. inversion H3. subst. now simpl.
+rewrite <- (app_nil_l s). autoIC.
+Qed. 
+
+Lemma seq_Failure : forall c s, s =~ Failure _;_ c <-> s =~ Failure.
+Proof.
+split;intros. inversion H. inversion H3. inversion H.
+Qed.
+
+Hint Resolve seq_Success seq_Failure : cDB.
+
+(*
+Lemma o_or : forall (c0 c1 : Contract)(s : Trace), s =~ o c0 _;_ c1 -> nu c0 = true /\ s =~ c1 \/ nu c0 = false /\ s =~ Failure.
+Proof.
+intros. o_destruct. unfold o in H. destruct (nu c0). funelim (o c0).
+- rewrite <- Heqcall in H. rewrite seq_Success in H. now left.
+- rewrite <- Heqcall in H. rewrite seq_Failure in H. now right.
+Qed.*)
+
+Lemma derive_distr_plus : forall (s : Trace)(c0 c1 : Contract), s \\ (c0 _+_ c1) = s \\ c0 _+_ s \\ c1.
+Proof.
+induction s;intros;simpl;auto.
+Qed. 
+
+Lemma o_true : forall (c: Contract), nu c = true -> o c = Success.
+Proof.
+intros. o_destruct;auto with cDB. rewrite H in H1. discriminate. 
+Qed.
+
+Lemma o_false : forall (c: Contract), nu c = false -> o c = Failure.
+Proof.
+intros. o_destruct. rewrite H in H1. discriminate. auto. 
+Qed.
+
+Hint Rewrite derive_distr_plus : cDB.
+
+Lemma nu_seq_derive : forall (e : EventType)(c0 c1 : Contract), 
+nu c0 = true -> nu (e \ c1) = true -> nu (e \ (c0 _;_ c1)) = true.
+Proof.
+intros. simpl. rewrite orb_true_iff. left. rewrite o_true;auto.
+Qed.
+
+(*Not needed*)
+(*
+Lemma nu_plus : forall c0 c1, nu (c0 _+_ c1) = true <-> nu c0 = true \/ nu c1 = true.
+Proof.
+intros. simpl. now rewrite orb_true_iff.
+Qed.*)
+
+Lemma nu_Failure : forall (s : Trace)(c : Contract), nu (s \\ (Failure _;_ c)) = false.
+Proof.
+induction s;intros. now simpl. simpl. rewrite o_false;auto.
+rewrite derive_distr_plus. simpl. now repeat rewrite IHs.
+Qed.
+
+Hint Rewrite nu_Failure : cDB.
+
+Lemma nu_Success : forall (s : Trace)(c : Contract), nu (s \\ (Success _;_ c)) = nu (s \\ c).
+Proof.
+induction s;intros;simpl;auto. 
+autorewrite with cDB using simpl;auto. rewrite orb_false_r. auto. 
+Qed.
+
+Hint Rewrite nu_Failure nu_Success : cDB.
+
+Lemma nu_seq_trace_derive : forall (s : Trace)(c0 c1 : Contract), 
+nu c0 = true -> nu (s \\ c1) = true -> nu (s \\ (c0 _;_ c1)) = true.
+Proof.
+induction s;intros;simpl in *. intuition.
+rewrite o_true;auto. rewrite derive_distr_plus. simpl. autorewrite with cDB.
+rewrite H0. btauto.
+Qed.
+
+Lemma matchesb_seq : forall (s0 s1 : Trace)(c0 c1 : Contract), nu (s0\\c0) = true -> nu (s1\\c1) = true -> nu ((s0++s1)\\(c0 _;_c1)) = true.
+Proof.
+induction s0;intros;simpl in *.
+- rewrite nu_seq_trace_derive; auto. 
+- autorewrite with cDB. simpl. rewrite orb_true_iff. right. 
+  rewrite IHs0;auto.
+Qed.
+
+Hint Rewrite matchesb_seq : cDB.
+
+Lemma nu_par_trace_derive_r : forall (s : Trace)(c0 c1 : Contract), 
+nu c0 = true -> nu (s \\ c1) = true -> nu (s \\ (c0 _*_ c1)) = true.
+Proof.
+induction s;intros;simpl in *. intuition.
+rewrite derive_distr_plus. simpl. rewrite (IHs c0);auto with bool.
+Qed.
+
+
+
+Lemma nu_par_trace_derive_l : forall (s : Trace)(c0 c1 : Contract), 
+nu c0 = true -> nu (s \\ c1) = true -> nu (s \\ (c1 _*_ c0)) = true.
+Proof.
+induction s;intros;simpl in *. intuition.
+rewrite derive_distr_plus. simpl. rewrite (IHs c0);auto with bool.
+Qed.
+
+Hint Resolve nu_par_trace_derive_l nu_par_trace_derive_r : cDB.
+
+Lemma matchesb_par : forall (s0 s1 s : Trace)(c0 c1 : Contract), interleave s0 s1 s ->
+nu (s0\\c0) = true -> nu (s1\\c1) = true -> nu (s\\(c0 _*_c1)) = true.
+Proof.
+intros. generalize dependent c1. generalize dependent c0.
+induction H;intros;simpl in*; auto with cDB. 
+- rewrite derive_distr_plus. simpl. rewrite IHinterleave;auto.
+- rewrite derive_distr_plus. simpl. rewrite (IHinterleave c0);auto with bool.
+Qed.
+
+
+Hint Resolve matchesb_par : cDB.
+
+
+Lemma Matches_Comp_i_matchesb : forall (c : Contract)(s : Trace), s =~ c -> nu (s\\c) = true.
+Proof.
+intros; induction H; 
+solve [ autorewrite with cDB; simpl; auto with bool 
+      | simpl;eq_event_destruct;eauto with cDB]. (*Only change: eauto, add matchesb_par*)
+Qed.
+
+
+
+Lemma Matches_Comp_nil_nu : forall (c : Contract), nu c = true -> [] =~ c.
+Proof.
+intros;induction c; simpl in H ; try discriminate; autoIC.
+- apply orb_prop in H. destruct H; autoIC.
+- rewrite <- (app_nil_l []); autoIC.
+- apply andb_prop in H. destruct H. eauto with cDB.
+Qed.
+
+
+(*This direction with longer trace on the right because of induction step on trace*)
+Lemma Matches_Comp_derive : forall (c : Contract)(e : EventType)(s : Trace), s =~ e \ c-> (e::s) =~ c.
+Proof.
+induction c;intros; simpl in*; try solve [inversion H].
+- eq_event_destruct. inversion H. subst. autoIC. inversion H.
+- inversion H; autoIC. (*apply IH directly*) 
+- inversion H.
+  * inversion H2. subst. o_destruct. 
+    inversion H7. simpl. 
+    rewrite <- (app_nil_l (e::s2)). constructor.
+    all: auto using Matches_Comp_nil_nu. 
+    inversion H7.
+  * inversion H1. subst. rewrite app_comm_cons. 
+    auto with cDB.
+- inversion H.
+  * inversion H2; subst; eauto with cDB.
+  * inversion H1;subst; eauto with cDB. (*New case*)
+Qed.
+
+
+
+
+Theorem Matches_Comp_iff_matchesb : forall (c : Contract)(s : Trace), s =~ c <-> nu (s \\ c) = true.
+Proof.
+split;intros.
+- auto using Matches_Comp_i_matchesb.
+- generalize dependent c. induction s;intros. 
+  simpl in H. auto using Matches_Comp_nil_nu.
+  auto using Matches_Comp_derive.
+Qed.
+
+Lemma derive_spec_comp : forall (c : Contract)(e : EventType)(s : Trace), e::s =~ c <-> s =~ e \ c.
+Proof.
+intros. repeat rewrite Matches_Comp_iff_matchesb. now simpl.
+Qed.
