theories/Parallel/ContractEquations.v
@@ -1,0 +1,592 @@
+Require Import CSL.Parallel.Contract.  
+Require Import Lists.List Bool.Bool Bool.Sumbool Setoid Coq.Arith.PeanoNat.
+From Equations Require Import Equations.
+Require Import micromega.Lia.
+(** printing =~ %$=\sim$% *)
+
+(** printing _+_ %$+$% *)
+
+Import ListNotations.
+
+Set Implicit Arguments.
+
+Reserved Notation "c0 =R= c1" (at level 63).
+
+Inductive c_eq : Contract -> Contract -> Prop :=
+  | c_plus_assoc c0 c1 c2 : (c0 _+_ c1) _+_ c2 =R= c0 _+_ (c1 _+_ c2)
+  | c_plus_comm c0 c1: c0 _+_ c1 =R= c1 _+_ c0
+  | c_plus_neut c: c _+_ Failure =R= c
+  | c_plus_idemp c : c _+_ c =R= c 
+  | c_seq_assoc c0 c1 c2 : (c0 _;_ c1) _;_ c2 =R= c0 _;_ (c1 _;_ c2)
+  | c_seq_neut_l c : (Success _;_ c) =R= c 
+  | c_seq_neut_r c : c _;_ Success =R= c 
+  | c_seq_failure_l c : Failure _;_ c =R= Failure    
+  | c_seq_failure_r c :  c _;_ Failure =R= Failure 
+  | c_distr_l c0 c1 c2 : c0 _;_ (c1 _+_ c2) =R= (c0 _;_ c1) _+_ (c0 _;_ c2)
+  | c_distr_r c0 c1 c2 : (c0 _+_ c1) _;_ c2 =R= (c0 _;_ c2) _+_ (c1 _;_ c2)
+
+  | c_par_assoc c0 c1 c2 : (c0 _*_ c1) _*_ c2 =R= c0 _*_ (c1 _*_ c2)
+  | c_par_neut c : c _*_ Success =R= c 
+  | c_par_comm c0 c1: c0 _*_ c1 =R= c1 _*_ c0
+  | c_par_failure c : c _*_ Failure =R= Failure   
+  | c_par_distr_l c0 c1 c2 : c0 _*_ (c1 _+_ c2) =R= (c0 _*_ c1) _+_ (c0 _*_ c2)
+
+  | c_par_event e0 e1 c0 c1 : Event e0 _;_ c0 _*_ Event e1 _;_ c1 =R= Event e0 _;_ (c0 _*_ (Event e1 _;_ c1)) _+_ Event e1 _;_ ((Event e0 _;_ c0) _*_ c1)
+
+  | c_refl c : c =R= c
+  | c_sym c0 c1 (H: c0 =R= c1) : c1 =R= c0
+  | c_trans c0 c1 c2 (H1 : c0 =R= c1) (H2 : c1 =R= c2) : c0 =R= c2
+  | c_plus_ctx c0 c0' c1 c1' (H1 : c0 =R= c0') (H2 : c1 =R= c1') : c0 _+_ c1 =R= c0' _+_ c1'
+  | c_seq_ctx c0 c0' c1 c1' (H1 : c0 =R= c0') (H2 : c1 =R= c1') : c0 _;_ c1 =R= c0' _;_ c1'
+  | c_par_ctx c0 c0' c1 c1' (H1 : c0 =R= c0') (H2 : c1 =R= c1') : c0 _*_ c1 =R= c0' _*_ c1'
+  where "c1 =R= c2" := (c_eq c1 c2).
+
+Hint Constructors c_eq : eqDB.
+
+Add Parametric Relation : Contract c_eq
+  reflexivity proved by c_refl
+  symmetry proved by c_sym
+  transitivity proved by c_trans
+  as Contract_setoid.
+
+Add Parametric Morphism : CPlus with
+signature c_eq ==> c_eq ==> c_eq as c_eq_plus_morphism.
+Proof.
+  intros. auto with eqDB.
+Qed.
+
+Add Parametric Morphism : CSeq with
+signature c_eq ==> c_eq ==> c_eq as c_eq_seq_morphism.
+Proof.
+  intros. auto with eqDB.
+Qed.
+
+Add Parametric Morphism : Par with
+signature c_eq ==> c_eq ==> c_eq as c_eq_par_morphism.
+Proof.
+  intros. auto with eqDB.
+Qed.
+
+
+Ltac c_inversion :=
+  (repeat match goal with
+         | [ H: _ =~ Failure |- _ ] => inversion H
+         | [ H: ?s =~ _ _+_ _ |- _ ] => inversion H; clear H
+         | [ H: ?s =~ _ _;_ _ |- _ ] => inversion H; clear H
+         | [ H: ?s =~ _ _*_ _ |- _ ] => inversion H; clear H
+         | [ H: [?x] =~ Event _ |- _ ] => fail
+         | [ H: ?s =~ Event _ |- _ ] => inversion H; subst
+         | [ H: [] =~ Success |- _ ] => fail
+         | [ H: _ =~ Success |- _ ] => inversion H; clear H
+         end);auto with cDB.
+
+
+
+
+Ltac interl_tac := 
+        (repeat match goal with
+         | [ H: _::_ = [] |- _ ] => discriminate
+         | [ H: _ /\ _ |- _ ] => destruct H
+         | [ H: _ \/ _ |- _ ] => destruct H
+         | [ H: interleave_fun _ _ [] |- _ ] => simpl in H
+         | [ H: interleave_fun _ _ (?e::?s) |- _ ] => simpl in H
+         | [ H: interleave_fun _ _ ?s |- _ ] => destruct s;simpl in H
+         | [ H: interleave _ _ _ |- _ ] => rewrite interl_iff_fun in H
+         end);subst.
+
+Lemma cons_app : forall (A: Type) (a : A)(l : list A), a::l = [a]++l.
+Proof. auto.
+Qed.
+
+Lemma event_seq : forall s e0 c0 e1 c1, s =~ (Event e0 _;_ c0) _*_ (Event e1 _;_ c1) <-> 
+s =~ Event e0 _;_ (c0 _*_ (Event e1 _;_ c1)) _+_ Event e1 _;_ ((Event e0 _;_ c0) _*_ c1).
+Proof.
+split;intros.
+- c_inversion. inversion H5;subst. symmetry in H1. apply app_eq_nil in H1.
+  destruct H1;subst;simpl. inversion H8. 
+  *  apply MPlusL. rewrite cons_app. constructor;auto.
+     econstructor;eauto. auto with cDB. 
+  * inversion H8;subst. simpl in H. inversion H. 
+    apply MPlusR. rewrite cons_app. constructor;auto;subst. 
+     econstructor;eauto. eapply MSeq;eauto.
+- c_inversion.
+  * inversion H6;subst. econstructor. econstructor;eauto. 
+    econstructor;eauto. simpl in*;auto with cDB.
+  * inversion H6;subst. econstructor. econstructor;eauto. 
+    econstructor;eauto. simpl in*;auto with cDB.
+Qed.
+
+Lemma c_eq_soundness : forall (c0 c1 : Contract), c0 =R= c1 -> (forall s : Trace, s =~ c0 <-> s =~ c1).
+Proof.
+intros c0 c1 H. induction H ;intros; try solve [split;intros;c_inversion].
+  * split;intros;c_inversion; [ rewrite <- app_assoc | rewrite app_assoc ]; auto with cDB.
+  * rewrite <- (app_nil_l s). split;intros;c_inversion.
+  * rewrite <- (app_nil_r s) at 1. split;intros;c_inversion. subst.
+    repeat rewrite app_nil_r in H1. now rewrite <- H1.
+  * split;intros; inversion H; subst.  (*new*)
+    ** inversion H3. subst. eapply interl_app in H5;eauto. destruct_ctx.
+       eauto with cDB.
+    ** inversion H4. subst. eapply interl_comm in H5. eapply interl_comm in H8.
+       eapply interl_app in H5;eauto. destruct_ctx. econstructor;eauto. 
+       econstructor;eauto. all: eauto using interl_comm.
+  * split;intros.
+    ** inversion H. subst. inversion H4. subst.
+       apply interl_eq_r in H5. subst;auto.
+    ** eauto with cDB. 
+  * split;intros.
+    ** inversion H. subst. econstructor;eauto using interl_comm.
+    ** inversion H. subst. econstructor;eauto using interl_comm.
+  * split;intros.
+    ** inversion H. subst. inversion H4;  eauto with cDB. 
+    ** inversion H. subst.
+      *** inversion H2. subst. econstructor;eauto with cDB. 
+      *** inversion H1. subst. econstructor;eauto with cDB. (*new*)
+  * apply event_seq.
+  * now symmetry.
+  * eauto using iff_trans.
+  * split;intros; inversion H1; [ rewrite IHc_eq1 in H4 
+                                | rewrite IHc_eq2 in H4
+                                | rewrite <- IHc_eq1 in H4 
+                                | rewrite <- IHc_eq2 in H4];auto with cDB.
+  * split;intros; c_inversion; constructor;
+                                [ rewrite <- IHc_eq1
+                                | rewrite <- IHc_eq2
+                                | rewrite IHc_eq1
+                                | rewrite IHc_eq2];auto.
+  * split;intros; c_inversion; econstructor;eauto;
+                                [ rewrite <- IHc_eq1
+                                | rewrite <- IHc_eq2
+                                | rewrite IHc_eq1
+                                | rewrite IHc_eq2];auto.
+Qed.
+
+Lemma Matches_plus_comm : forall c0 c1 s, s =~ c0 _+_ c1 <-> s =~ c1 _+_ c0.
+Proof. auto using c_eq_soundness  with eqDB. Qed.
+
+Lemma Matches_plus_neut_l : forall c s, s =~ Failure _+_ c <-> s =~ c.
+Proof. intros. rewrite Matches_plus_comm. auto using c_eq_soundness  with eqDB. Qed.
+
+Lemma Matches_plus_neut_r : forall c s, s =~ c _+_ Failure <-> s =~ c.
+Proof. auto using c_eq_soundness  with eqDB. Qed.
+
+Lemma Matches_seq_neut_l : forall c s, s =~ (Success _;_ c) <-> s =~ c.
+Proof. auto using c_eq_soundness  with eqDB. Qed.
+
+Lemma Matches_seq_neut_r : forall c s, s =~ c _;_ Success <-> s =~ c.
+Proof. auto using c_eq_soundness  with eqDB. Qed.
+
+Lemma Matches_seq_assoc : forall c0 c1 c2 s, s =~ (c0 _;_ c1) _;_ c2  <-> s =~ c0 _;_ (c1 _;_ c2).
+Proof. auto using c_eq_soundness  with eqDB. Qed.
+
+Hint Rewrite Matches_plus_neut_l 
+             Matches_plus_neut_r 
+             Matches_seq_neut_l
+             Matches_seq_neut_r : eqDB.
+
+Lemma c_plus_neut_l : forall c, Failure _+_ c =R= c.
+Proof. intros. rewrite c_plus_comm. auto with eqDB.
+Qed.
+
+Hint Rewrite c_plus_neut_l 
+             c_plus_neut 
+             c_seq_neut_l
+             c_seq_neut_r
+             c_seq_failure_l 
+             c_seq_failure_r 
+             c_distr_l
+             c_distr_r : eqDB.
+
+Ltac auto_rwd_eqDB := autorewrite with eqDB;auto with eqDB.
+
+Equations interleavings  (s0 s1: Trace) : (list Trace) by  wf ((length s0) + (length s1)) :=
+interleavings [] s1 := [s1];
+interleavings s0 [] := [s0];
+interleavings (e0::s0') (e1::s1') := (map (fun s => e0::s) (interleavings s0' (e1::s1'))) ++ 
+                                     (map (fun s => e1::s) (interleavings (e0::s0') s1')).
+Next Obligation.  lia. Defined.
+
+Theorem interleavings_i_interleave_fun : forall (s0 s1 s : Trace), In s (interleavings s0 s1) -> interleave_fun s0 s1 s.
+Proof.
+intros. funelim (interleavings s0 s1).
+- simp interleavings in H. simpl in H. destruct H;try contradiction. subst. auto with cDB.
+- simp interleavings in H. simpl in H. destruct H;try contradiction. subst. auto with cDB.
+- simp interleavings in H1. apply in_app_or in H1. destruct H1.
+  * rewrite in_map_iff in H1. destruct_ctx. apply H in H2. 
+    subst. auto with cDB.
+  * rewrite in_map_iff in H1. destruct_ctx. apply H0 in H2. 
+    subst. auto with cDB.
+Qed.
+
+Lemma in_one : forall (A:Type) (a a0 : A), In a [a0] -> a = a0.
+Proof.
+intros. simpl in H. destruct H;try contradiction;auto.
+Qed.
+
+Lemma interleavings_nil_r : forall s, interleavings s []  = [s].
+Proof.
+induction s;intros; reflexivity.
+Qed.
+
+Lemma interleavings_one_l : forall (s : Trace)e,  In (e :: s) (interleavings [e] s).
+Proof.
+intros. funelim (interleavings [e] s).
+-  simp interleavings. apply in_eq.
+- rewrite <- Heqcall. apply in_or_app. left. rewrite in_map_iff.
+  exists (e0::l0). split;auto. simp interleavings. apply in_eq.
+Qed.
+
+Lemma interleavings_one_r : forall (s : Trace)e,  In (e :: s) (interleavings s [e]).
+Proof.
+intros. funelim (interleavings s [e]).
+-  simp interleavings. apply in_eq.
+- rewrite <- Heqcall. apply in_or_app. right. rewrite in_map_iff.
+  exists (e::l). split;auto. simp interleavings. apply in_eq.
+Qed.
+
+Lemma interleavings_extend_l : forall (s0 s1 s : Trace) e,  In s (interleavings s0 s1) ->
+In (e::s) (interleavings (e::s0) s1).
+Proof. 
+intros. destruct s1. simp interleavings in*. rewrite interleavings_nil_r in *. 
+apply in_one in H. subst. apply in_eq. 
+simp interleavings. apply in_or_app. left. rewrite in_map_iff.
+exists s. split;auto.
+Qed.
+
+Lemma interleavings_extend_r : forall (s0 s1 s : Trace) e,  In s (interleavings s0 s1) ->
+In (e::s) (interleavings s0 (e::s1)).
+Proof. 
+intros. destruct s0. simp interleavings in*. apply in_one in H. subst.
+apply in_eq. 
+simp interleavings. apply in_or_app. right. rewrite in_map_iff.
+exists s. split;auto.
+Qed.
+
+Theorem interleave_fun_i_interleavings : forall (s s0 s1: Trace), interleave_fun s0 s1 s
+-> In s (interleavings s0 s1).
+Proof.
+induction s;intros. simpl in H. destruct H. subst. simpl. now left.
+simpl in H. destruct s0.
+- subst. simpl. now left.
+- destruct H.
+  * destruct H. subst. apply IHs in H0. auto using interleavings_extend_l.
+  * destruct s1.
+    ** simp interleavings. inversion H. apply in_eq.
+    ** destruct H. subst. apply IHs in H0. auto using interleavings_extend_r.
+Qed.
+
+Theorem interleave_fun_iff_interleavings : forall (s s0 s1: Trace),
+interleave_fun s0 s1 s <-> In s (interleavings s0 s1).
+Proof. split; auto using interleave_fun_i_interleavings, interleavings_i_interleave_fun.
+Qed.
+
+
+
+Fixpoint L (c : Contract) : list Trace :=
+match c with
+| Success => [[]]
+| Failure => []
+| Event e => [[e]]
+| c0 _+_ c1 => (L c0) ++ (L c1)
+| c0 _;_ c1 => map (fun p => (fst p)++(snd p)) (list_prod (L c0) (L c1))
+| c0 _*_ c1 => flat_map (fun p => interleavings (fst p) (snd p)) (list_prod (L c0) (L c1))
+end.
+
+
+Lemma Matches_member : forall (s : Trace)(c : Contract), s =~ c -> In s (L c). 
+Proof.
+intros. induction H ; simpl ; try solve [auto using in_or_app || auto using in_or_app ].
+- rewrite in_map_iff. exists (s1,s2). rewrite in_prod_iff. split;auto.
+- rewrite in_flat_map. exists (s1,s2). split.
+  * rewrite in_prod_iff. split;auto.
+  * simpl. rewrite <- interleave_fun_iff_interleavings. 
+    now rewrite <- interl_iff_fun.
+Qed.
+
+Lemma member_Matches : forall (c : Contract)(s : Trace), In s (L c) -> s =~ c. 
+Proof.
+induction c;intros;simpl in*; try solve [ destruct H;try contradiction; subst; constructor].
+- apply in_app_or in H. destruct H; auto with cDB.
+- rewrite in_map_iff in H. destruct_ctx. destruct x.
+  rewrite in_prod_iff in H0. destruct H0. simpl in H.
+  subst. auto with cDB.
+- rewrite in_flat_map in H. destruct_ctx.
+  rewrite <- interleave_fun_iff_interleavings in H0. 
+  destruct x. rewrite in_prod_iff in H. destruct H.
+  simpl in*. rewrite <- interl_iff_fun in H0. eauto with cDB.
+Qed.
+
+Theorem Matches_iff_member : forall s c, s =~ c <-> In s (L c).
+Proof.
+split; auto using Matches_member,member_Matches.
+Qed.
+
+Lemma Matches_incl : forall (c0 c1 : Contract), (forall (s : Trace), s =~ c0 -> s =~ c1) -> 
+incl (L c0) (L c1).
+Proof.
+intros. unfold incl. intros. rewrite <- Matches_iff_member in *. auto.
+Qed.
+
+Lemma comp_equiv_destruct : forall (c0 c1: Contract),(forall s : Trace, s =~ c0 <-> s =~ c1) <->
+(forall s : Trace, s =~ c0 -> s =~ c1) /\ (forall s : Trace, s =~ c1 -> s =~ c0).
+Proof.
+ split ; intros.
+- split;intros; specialize H with s; destruct H; auto.
+- destruct H. split;intros;auto.
+Qed.
+
+
+Theorem Matches_eq_i_incl_and : forall (c0 c1 : Contract), (forall (s : Trace), s =~ c0 <-> s =~ c1) -> 
+incl (L c0) (L c1) /\ incl (L c1) (L c0) .
+Proof.
+intros. apply comp_equiv_destruct in H. destruct H. split; auto using Matches_incl. 
+Qed.
+
+
+Fixpoint Σ (l : list Contract) : Contract :=
+match l with
+| [] => Failure
+| c ::l => c _+_ (Σ l)
+end.
+
+(*Maybe not needed*)
+Lemma Σ_app : forall (l1 l2 : list Contract), 
+Σ (l1 ++ l2) =R= (Σ l1) _+_ (Σ l2).
+Proof.
+induction l1;intros;simpl;auto_rwd_eqDB.
+rewrite IHl1. now rewrite c_plus_assoc.
+Qed.
+
+(*Not used in this file, maybe used in decision procedure*)
+Lemma in_Σ : forall (l : list Contract)(s : Trace), s =~ Σ l <-> 
+(exists c, In c l /\ s =~ c).
+Proof. 
+induction l;intros;simpl.
+- split;intros. c_inversion. destruct_ctx. contradiction.
+- split;intros. c_inversion. exists a. split;auto.
+  rewrite IHl in H1. destruct_ctx. exists x. split;auto.
+  destruct_ctx. inversion H. subst. auto with cDB.
+  apply MPlusR. rewrite IHl. exists x. split;auto.
+Qed.
+
+Lemma in_Σ_idemp : forall l c, In c l -> c _+_ Σ l =R= Σ l.
+Proof.
+induction l;intros;simpl; auto_rwd_eqDB.
+simpl in H;contradiction.
+simpl in H. destruct H. subst. all: rewrite <- c_plus_assoc.
+auto_rwd_eqDB. rewrite (c_plus_comm c). rewrite c_plus_assoc. 
+apply c_plus_ctx;auto_rwd_eqDB.
+Qed. 
+
+Lemma incl_Σ_idemp : forall (l1 l2 : list Contract), incl l1 l2 -> Σ l2 =R= Σ (l1++l2).
+Proof. 
+induction l1;intros;simpl;auto_rwd_eqDB.
+apply incl_cons_inv in H as [H0 H1].
+rewrite <- IHl1;auto. now rewrite in_Σ_idemp;auto.
+Qed.
+
+Lemma Σ_app_comm : forall (l1 l2 : list Contract), Σ (l1++l2) =R= Σ (l2++l1).
+Proof.
+induction l1;intros;simpl. now rewrite app_nil_r.
+repeat rewrite Σ_app. rewrite <- c_plus_assoc.
+rewrite c_plus_comm. apply c_plus_ctx;auto_rwd_eqDB.
+Qed.
+
+Lemma incl_Σ_c_eq : forall (l1 l2 : list Contract), incl l1 l2 -> incl l2 l1-> Σ l1 =R= Σ l2.
+Proof.
+intros. rewrite (incl_Σ_idemp H). 
+rewrite (incl_Σ_idemp H0). apply Σ_app_comm.
+Qed.
+
+
+Fixpoint Π (s : Trace) :=
+match s with
+| [] => Success
+| e::s' => (Event e) _;_ (Π s')
+end.
+
+Lemma Π_app : forall (l1 l2 : Trace), Π l1 _;_ Π l2 =R= Π (l1++l2).
+Proof.
+induction l1;intros;simpl; auto_rwd_eqDB.
+rewrite <- IHl1. auto_rwd_eqDB.
+Qed.
+
+(*
+Definition Π (l : list Trace) := Σ (map Π l).
+Hint Unfold Π : eqDB.*)
+
+
+Lemma Π_distr_aux : forall (ss : list Trace) (s : Trace), Π s _;_ (Σ (map Π ss)) =R=
+ Σ (map (fun x => Π (fst x ++ snd x)) (map (fun y : list EventType => (s, y)) ss)).
+Proof.
+induction ss;intros;simpl;auto_rwd_eqDB.
+apply c_plus_ctx;auto using Π_app.
+Qed.
+
+Lemma Π_distr_aux2 : forall c l0, c _;_ Σ (map Π l0) =R=
+ Σ (map (fun x => c _;_ Π x) l0).
+Proof.
+induction l0;intros;simpl;auto_rwd_eqDB.
+Qed.
+
+
+(*
+Lemma Π_distr2 : forall l0 l1,  Σ l0 _;_ Σ l1 =R=
+ Σ (map (fun x => (fst x) _;_ (snd x)) (list_prod l0 l1)).
+Proof.
+induction l0;intros;simpl. auto_rwd_eqDB.
+repeat rewrite map_app. rewrite Σ_app. rewrite <- IHl0.
+auto_rwd_eqDB. rewrite map_map. simpl. 
+apply c_plus_ctx; auto using Π_distr_aux2 with eqDB. 
+Qed.*)
+
+(*Mention in report*)
+Lemma map_ext_in_R :
+  forall (A : Type)(f g:A->Contract) l, (forall a, In a l -> f a =R= g a) -> Σ (map f l) =R= Σ (map g l).
+Proof.
+induction l;intros;simpl;auto with eqDB.
+apply c_plus_ctx. apply H. apply in_eq. apply IHl.
+intros. apply H. simpl. now right.
+Qed.
+
+Lemma exchange : forall p q r s, 
+ (p _*_ q) _;_ (r _*_ s) _+_ (p _;_ r) _*_ (q _;_ s) =R= (p _;_ r) _*_ (q _;_ s).
+Proof. Admitted.
+
+Lemma exchange2 : forall a b c, 
+ a _*_ (b _;_ c) _+_ (a _*_ b) _;_ c =R=
+ a _*_ (b _;_ c).
+Proof. Admitted.
+
+
+(*
+Lemma Π_par_aux2 : forall (s0 s1 : Trace) e, Event e _;_ Π s0 _*_ Π s1 =R=
+ Σ (map (fun x => Π (e::x)) (interleavings s0 s1)).
+Proof.
+intros. simpl. rewrite <- Π_distr_aux2. 
+apply c_seq_ctx. auto with eqDB.*)
+
+Lemma Σ_interleavings : forall (s0 s1 : Trace),
+Σ (map Π (interleavings s0 s1)) =R= (Π s0) _*_ (Π s1).
+Proof.
+intros. funelim (interleavings s0 s1).
+- simp interleavings. simpl. rewrite c_par_comm. auto_rwd_eqDB.
+- rewrite interleavings_nil_r. simpl. auto_rwd_eqDB.
+- simp interleavings. rewrite map_app. rewrite Σ_app.
+  repeat rewrite map_map. clear Heqcall. simpl.
+  repeat rewrite <- Π_distr_aux2. rewrite H.
+  rewrite H0. simpl.
+
+  remember ( Π l) as c. remember (Π l0) as d.
+  now rewrite c_par_event.
+Qed.
+
+
+Lemma Π_distr : forall l0 l1,  Σ (map Π l0) _;_ Σ (map Π l1) =R=
+ Σ (map (fun x => Π (fst x ++ snd x)) (list_prod l0 l1)).
+Proof.
+induction l0;intros;simpl. auto_rwd_eqDB.
+repeat rewrite map_app. rewrite Σ_app. rewrite <- IHl0.
+auto_rwd_eqDB. 
+apply c_plus_ctx; auto using Π_distr_aux with eqDB. 
+Qed.
+
+(*
+
+
+Lemma Σ_interleavings_aux : forall (s0 s1 : Trace) c,
+Σ (map (fun x => c _;_ Π x) (interleavings s0 s1)) =R= c _;_ ((Π s0) _*_ (Π s1)).
+Proof.
+intros. funelim (interleavings s0 s1).
+- simp interleavings. simpl. rewrite c_par_comm. auto_rwd_eqDB.
+- rewrite interleavings_nil_r. simpl. auto_rwd_eqDB.
+- simp interleavings. rewrite map_app.
+  rewrite Σ_app. rewrite map_map.
+  rewrite map_ext_in_R.
+  * rewrite H. rewrite map_map. simpl. rewrite map_ext_in_R.
+    ** rewrite H0. simpl.
+  setoid_rewrite <- c_seq_assoc. rewrite H0.
+
+ rewrite <- c_seq_neut. rewrite <- exchange. rewrite <- par_der. reflexivity. auto with eqDB. apply par_der.  rewrite simpl in H0. rewrite 
+  rewrite map_map. simpl.
+  rewrite <- H.
+*)
+
+
+
+Lemma Π_par_aux : forall (ss : list Trace) (s : Trace), Π s _*_ (Σ (map Π ss)) =R=
+ Σ (map Π (flat_map (fun x => interleavings (fst x) (snd x)) (map (fun y : list EventType => (s, y)) ss))).
+Proof.
+induction ss;intros;simpl;auto_rwd_eqDB.
+rewrite map_app. rewrite Σ_app. rewrite <- IHss.
+rewrite c_par_distr_l. rewrite Σ_interleavings. auto with eqDB.
+Qed.
+
+
+Lemma Π_distr_par : forall l0 l1,  Σ (map Π l0) _*_ Σ (map Π l1) =R=
+ Σ (map Π (flat_map (fun x =>(interleavings (fst x) (snd x))) (list_prod l0 l1))).
+Proof.
+induction l0;intros;simpl. rewrite c_par_comm. auto_rwd_eqDB.
+rewrite flat_map_app. rewrite map_app. rewrite  Σ_app.
+rewrite <- IHl0. rewrite <- Π_par_aux. 
+rewrite c_par_comm. rewrite c_par_distr_l.
+ auto with eqDB. 
+Qed.
+
+
+
+Theorem Π_L_ceq : forall (c : Contract), Σ (map Π (L c)) =R= c.
+Proof.
+induction c; simpl; try solve [auto_rwd_eqDB].
+- rewrite map_app. rewrite Σ_app.
+  auto using c_plus_ctx. 
+- rewrite map_map.
+  rewrite <- IHc1 at 2. rewrite <- IHc2 at 2.
+  symmetry. apply Π_distr.
+- rewrite <- IHc1 at 2. rewrite <- IHc2 at 2.
+  rewrite Π_distr_par. auto with eqDB.
+Qed.
+
+
+
+Lemma c_eq_completeness : forall (c0 c1 : Contract), (forall s : Trace, s =~ c0 <-> s =~ c1) -> c0 =R= c1.
+Proof.
+intros. rewrite <- Π_L_ceq. rewrite <- (Π_L_ceq c1). 
+apply Matches_eq_i_incl_and in H.
+destruct H. auto using incl_map, incl_Σ_c_eq.
+Qed.
+
+
+
+Theorem Matches_iff_c_eq : forall c0 c1, (forall s, s =~ c0 <-> s =~ c1) <-> c0 =R= c1.
+Proof.
+split; auto using c_eq_completeness, c_eq_soundness.
+Qed.
+
+Lemma L_Σ : forall l, L (Σ l) = flat_map L l.
+Proof.
+induction l;intros;simpl;auto. now rewrite IHl.
+Qed.
+
+
+
+
+
+
+
+
+
+
+
+
+
+
+
+
+
+
+
+
+
+
+
+ 
